error.bpl
@@ -1,0 +1,412 @@
+type Ref;
+
+type Field _;
+
+const unique zero: Ref;
+
+const unique OptIn: int;
+
+const unique Noop: int;
+
+const unique CloseOut: int;
+
+var Alloc: [Ref]bool;
+
+var Globals: [Ref]Ref;
+
+var GlobalsAlloc: [Ref]bool;
+
+var ScratchSpace: [int]Ref;
+
+var ScratchSpaceAlloc: [int]bool;
+
+var StackPointer: int;
+
+var Stack: [int]Ref;
+
+var IsInt: [Ref]bool;
+
+var RefToInt: [Ref]int;
+
+var CurrentTxn: Ref;
+
+var Sender: [Ref]Ref;
+
+var NumAppArgs: [Ref]Ref;
+
+var ApplicationArgs: [Ref][int]Ref;
+
+var OnCompletion: [Ref]Ref;
+
+var Accounts: [Ref][int]Ref;
+
+var GroupTransaction: [Ref][int]Ref;
+
+var ApplicationID: [Ref]Ref;
+
+var TypeEnum: [Ref]Ref;
+
+var AssetReceiver: [Ref]Ref;
+
+var XferAsset: [Ref]Ref;
+
+var AssetAmount: [Ref]Ref;
+
+procedure FreshRefGenerator() returns (newRef: Ref);
+  modifies Alloc, IsInt;
+  ensures old(Alloc[newRef] <==> false);
+  ensures Alloc[newRef] <==> true;
+  ensures newRef != zero;
+  ensures IsInt[newRef] <==> false;
+  ensures (forall ref: Ref :: ref != newRef ==> (IsInt[ref] <==> old(IsInt[ref])));
+  ensures (forall ref: Ref :: ref != newRef ==> (Alloc[ref] <==> old(Alloc[ref])));
+
+
+
+implementation FreshRefGenerator() returns (newRef: Ref)
+{
+
+  anon0:
+    havoc newRef;
+    assume Alloc[newRef] <==> false;
+    Alloc[newRef] := true;
+    IsInt[newRef] := false;
+    assume newRef != zero;
+    return;
+}
+
+
+
+procedure Push(value: Ref);
+  modifies StackPointer, Stack;
+  ensures old(StackPointer) + 1 == StackPointer;
+  ensures Stack[StackPointer] == value;
+  ensures (forall i: int :: -1 <= i && i < StackPointer ==> Stack[i] == old(Stack[i]));
+
+
+
+implementation Push(value: Ref)
+{
+
+  anon0:
+    StackPointer := StackPointer + 1;
+    Stack[StackPointer] := value;
+    return;
+}
+
+
+
+procedure Pop() returns (top: Ref);
+  requires StackPointer >= 0;
+  modifies StackPointer;
+  ensures StackPointer == old(StackPointer) - 1;
+  ensures top == old(Stack[old(StackPointer)]);
+
+
+
+implementation Pop() returns (top: Ref)
+{
+
+  anon0:
+    top := Stack[StackPointer];
+    StackPointer := StackPointer - 1;
+    return;
+}
+
+
+
+procedure Store(i: int);
+  requires 0 <= i;
+  requires i < 64;
+  requires StackPointer >= 0;
+  modifies ScratchSpace, ScratchSpaceAlloc, Stack, StackPointer;
+  ensures ScratchSpaceAlloc[i] <==> true;
+  ensures ScratchSpace[i] == Stack[old(StackPointer)];
+  ensures StackPointer == old(StackPointer) - 1;
+  ensures (forall j: int :: -1 <= j && j <= StackPointer ==> Stack[j] == old(Stack[j]));
+  ensures (forall j: int :: 0 < j && j < 64 && i != j ==> ScratchSpace[j] == old(ScratchSpace[j]));
+  ensures (forall j: int :: 0 < j && j < 64 && i != j ==> (ScratchSpaceAlloc[j] <==> old(ScratchSpaceAlloc[j])));
+
+
+
+procedure Load(i: int);
+  requires 0 <= i;
+  requires i < 64;
+  requires ScratchSpaceAlloc[i] <==> true;
+  modifies Stack, StackPointer;
+  ensures Stack[StackPointer] == ScratchSpace[i];
+  ensures StackPointer == old(StackPointer) + 1;
+  ensures (forall j: int :: -1 <= j && j < StackPointer ==> Stack[j] == old(Stack[j]));
+  ensures (forall j: int :: 0 < j && j < 64 && i != j ==> (ScratchSpaceAlloc[j] <==> old(ScratchSpaceAlloc[j])));
+
+
+
+procedure AppGlobalGet();
+  requires StackPointer >= 0;
+  modifies Stack, StackPointer;
+  ensures ((GlobalsAlloc[old(Stack)[old(StackPointer)]] <==> true) && Stack[StackPointer] == Globals[old(Stack)[old(StackPointer)]]) || Stack[StackPointer] == zero;
+  ensures StackPointer == old(StackPointer);
+  ensures (forall i: int :: -1 <= i && i < StackPointer ==> Stack[i] == old(Stack[i]));
+
+
+
+procedure AppGlobalPut();
+  requires StackPointer > 0;
+  modifies StackPointer, GlobalsAlloc, Globals;
+  ensures GlobalsAlloc[old(Stack[old(StackPointer) - 1])] <==> true;
+  ensures Globals[old(Stack[old(StackPointer) - 1])] == old(Stack[old(StackPointer)]);
+  ensures StackPointer == old(StackPointer) - 2;
+  ensures (forall i: int :: -1 <= i && i <= StackPointer ==> Stack[i] == old(Stack[i]));
+  ensures (forall ref: Ref :: ref != old(Stack[old(StackPointer) - 1]) ==> Globals[ref] == old(Globals[ref]));
+  ensures (forall ref: Ref :: ref != old(Stack[old(StackPointer) - 1]) ==> (GlobalsAlloc[ref] <==> old(GlobalsAlloc[ref])));
+
+
+
+implementation AppGlobalPut()
+{
+  var value: Ref;
+  var key: Ref;
+
+  anon0:
+    call {:si_unique_call 0} value := Pop();
+    call {:si_unique_call 1} key := Pop();
+    GlobalsAlloc[key] := true;
+    Globals[key] := value;
+    return;
+}
+
+
+
+procedure Dup();
+  requires StackPointer >= 0;
+  modifies Stack, StackPointer;
+  ensures Stack[old(StackPointer)] == old(Stack[old(StackPointer)]);
+  ensures Stack[StackPointer] == old(Stack[old(StackPointer)]);
+  ensures StackPointer == old(StackPointer) + 1;
+  ensures (forall i: int :: -1 <= i && i < StackPointer ==> Stack[i] == old(Stack[i]));
+
+
+
+procedure Int(n: int);
+  requires n >= 0;
+  modifies Alloc, IsInt, RefToInt, StackPointer, Stack;
+  ensures IsInt[Stack[StackPointer]];
+  ensures RefToInt[Stack[StackPointer]] == n;
+  ensures StackPointer == old(StackPointer) + 1;
+  ensures (forall i: int :: -1 <= i && i < StackPointer ==> Stack[i] == old(Stack[i]));
+  ensures (forall ref: Ref :: ref != Stack[StackPointer] ==> RefToInt[ref] == old(RefToInt[ref]));
+  ensures (forall ref: Ref :: ref != Stack[StackPointer] ==> (IsInt[ref] <==> old(IsInt[ref])));
+  ensures (forall ref: Ref :: ref != Stack[StackPointer] ==> (Alloc[ref] <==> old(Alloc[ref])));
+
+
+
+implementation Int(n: int)
+{
+  var newRef: Ref;
+
+  anon0:
+    call {:si_unique_call 2} newRef := FreshRefGenerator();
+    IsInt[newRef] := true;
+    RefToInt[newRef] := n;
+    call {:si_unique_call 3} Push(newRef);
+    return;
+}
+
+
+
+procedure Sum();
+  requires StackPointer > 0;
+  requires IsInt[Stack[StackPointer]];
+  requires IsInt[Stack[StackPointer - 1]];
+  requires RefToInt[Stack[StackPointer]] >= 0;
+  requires RefToInt[Stack[StackPointer - 1]] >= 0;
+  modifies IsInt, Alloc, StackPointer, Stack, RefToInt;
+  ensures RefToInt[Stack[StackPointer]] == old(RefToInt[old(Stack[old(StackPointer)])]) + old(RefToInt[old(Stack[old(StackPointer) - 1])]);
+  ensures StackPointer == old(StackPointer) - 1;
+  ensures (forall i: int :: -1 <= i && i < StackPointer ==> Stack[i] == old(Stack[i]));
+  ensures (forall ref: Ref :: ref != old(Stack[old(StackPointer)]) && ref != old(Stack[old(StackPointer) - 1]) && ref != Stack[StackPointer] ==> RefToInt[ref] == old(RefToInt[ref]));
+  ensures (forall ref: Ref :: ref != old(Stack[old(StackPointer)]) && ref != old(Stack[old(StackPointer) - 1]) && ref != Stack[StackPointer] ==> (IsInt[ref] <==> old(IsInt[ref])));
+
+
+
+procedure Byte(ref: Ref);
+  requires ref != zero;
+  requires IsInt[ref] <==> false;
+  modifies StackPointer, Stack;
+  ensures IsInt[ref] <==> false;
+  ensures Stack[StackPointer] == ref;
+  ensures StackPointer == old(StackPointer) + 1;
+  ensures (forall i: int :: -1 <= i && i < StackPointer ==> Stack[i] == old(Stack[i]));
+  ensures (forall ref': Ref :: ref != ref' ==> (IsInt[ref'] <==> old(IsInt[ref'])));
+  ensures (forall ref': Ref :: ref != ref' ==> (Alloc[ref'] <==> old(Alloc[ref'])));
+
+
+
+implementation Byte(ref: Ref)
+{
+
+  anon0:
+    call {:si_unique_call 4} Push(ref);
+    return;
+}
+
+
+
+procedure Return();
+  requires !IsInt[Stack[StackPointer]] || RefToInt[Stack[StackPointer]] > 0;
+
+
+
+implementation Return()
+{
+
+  anon0:
+    return;
+}
+
+
+
+procedure Txn(field: [Ref]Ref);
+  modifies StackPointer, Stack;
+  ensures StackPointer == old(StackPointer) + 1;
+  ensures Stack[StackPointer] == field[CurrentTxn];
+  ensures (forall i: int :: -1 <= i && i < StackPointer ==> Stack[i] == old(Stack[i]));
+
+
+
+implementation Txn(field: [Ref]Ref)
+{
+
+  anon0:
+    call {:si_unique_call 5} Push(field[CurrentTxn]);
+    return;
+}
+
+
+
+procedure Equal();
+  requires StackPointer > 0;
+  requires Stack[StackPointer] == zero || Stack[StackPointer - 1] == zero || (IsInt[Stack[StackPointer]] <==> IsInt[Stack[StackPointer - 1]]);
+  modifies StackPointer, Alloc, IsInt, RefToInt, Stack;
+  ensures StackPointer == old(StackPointer - 1);
+  ensures IsInt[Stack[StackPointer]];
+  ensures RefToInt[Stack[StackPointer]] == 1 || RefToInt[Stack[StackPointer]] == 0;
+  ensures old(Stack[StackPointer]) == old(Stack[StackPointer - 1]) ==> RefToInt[Stack[StackPointer]] == 1;
+  ensures old(IsInt[Stack[StackPointer]]) && old(IsInt[Stack[StackPointer - 1]]) && old(RefToInt[Stack[StackPointer]]) == old(RefToInt[Stack[StackPointer - 1]]) ==> RefToInt[Stack[StackPointer]] == 1;
+  ensures (forall ref': Ref :: Stack[StackPointer] != ref' ==> (IsInt[ref'] <==> old(IsInt[ref'])));
+  ensures (forall ref': Ref :: Stack[StackPointer] != ref' ==> RefToInt[ref'] == old(RefToInt[ref']));
+  ensures (forall ref': Ref :: Stack[StackPointer] != ref' ==> (Alloc[ref'] <==> old(Alloc[ref'])));
+  ensures (forall i: int :: -1 <= i && i < StackPointer ==> Stack[i] == old(Stack[i]));
+
+
+
+implementation Equal()
+{
+  var aRef: Ref;
+  var bRef: Ref;
+
+  anon0:
+    call {:si_unique_call 6} aRef := Pop();
+    call {:si_unique_call 7} bRef := Pop();
+    goto anon3_Then, anon3_Else;
+
+  anon3_Then:
+    assume {:partition} aRef == bRef || (IsInt[aRef] && RefToInt[aRef] == RefToInt[bRef]);
+    call {:si_unique_call 8} Int(1);
+    return;
+
+  anon3_Else:
+    assume {:partition} !(aRef == bRef || (IsInt[aRef] && RefToInt[aRef] == RefToInt[bRef]));
+    goto anon2;
+
+  anon2:
+    call {:si_unique_call 9} Int(0);
+    return;
+}
+
+
+
+procedure contract();
+  requires StackPointer == -1;
+  requires (forall ref: Ref :: IsInt[ref] <==> false);
+  requires (forall ref: Ref :: GlobalsAlloc[ref] <==> false);
+  requires (forall ref: Ref :: Alloc[ref] <==> false);
+  requires (forall i: int :: ScratchSpaceAlloc[i] <==> false);
+  requires (forall i: int :: Stack[i] == zero);
+  modifies IsInt, RefToInt, ApplicationID, Alloc, StackPointer, Stack, GlobalsAlloc, Globals;
+
+
+
+implementation contract()
+{
+  var creator: Ref;
+  var regBegin: Ref;
+  var regEnd: Ref;
+  var voteBegin: Ref;
+  var voteEnd: Ref;
+  var register: Ref;
+  var vote: Ref;
+  var voted: Ref;
+  var candidatea: Ref;
+  var candidateb: Ref;
+
+  anon0:
+    IsInt[zero] := true;
+    RefToInt[zero] := 0;
+    ApplicationID[CurrentTxn] := zero;
+    call {:si_unique_call 10} creator := FreshRefGenerator();
+    call {:si_unique_call 11} regBegin := FreshRefGenerator();
+    call {:si_unique_call 12} regEnd := FreshRefGenerator();
+    call {:si_unique_call 13} voteBegin := FreshRefGenerator();
+    call {:si_unique_call 14} voteEnd := FreshRefGenerator();
+    call {:si_unique_call 15} register := FreshRefGenerator();
+    call {:si_unique_call 16} vote := FreshRefGenerator();
+    call {:si_unique_call 17} voted := FreshRefGenerator();
+    call {:si_unique_call 18} candidatea := FreshRefGenerator();
+    call {:si_unique_call 19} candidateb := FreshRefGenerator();
+    assert Stack[StackPointer] != creator;
+    call {:si_unique_call 20} Int(0);
+    assert Stack[StackPointer] != creator;
+    call {:si_unique_call 21} Txn(ApplicationID);
+    call {:si_unique_call 22} Equal();
+    goto anon4_Then, anon4_Else;
+
+  anon4_Then:
+    assume {:partition} IsInt[Stack[StackPointer]] && RefToInt[Stack[StackPointer]] == 0;
+    goto failed;
+
+  anon4_Else:
+    assume {:partition} !(IsInt[Stack[StackPointer]] && RefToInt[Stack[StackPointer]] == 0);
+    goto anon2;
+
+  anon2:
+    call {:si_unique_call 23} Byte(creator);
+    call {:si_unique_call 24} Txn(Sender);
+    call {:si_unique_call 25} AppGlobalPut();
+    assume IsInt[NumAppArgs] <==> true;
+    assume RefToInt[NumAppArgs] == 4;
+    call {:si_unique_call 26} Txn(NumAppArgs);
+    call {:si_unique_call 27} Int(4);
+    call {:si_unique_call 28} Equal();
+    goto anon5_Then, anon5_Else;
+
+  anon5_Then:
+    assume {:partition} IsInt[Stack[StackPointer]] && RefToInt[Stack[StackPointer]] == 0;
+    goto failed;
+
+  anon5_Else:
+    assume {:partition} !(IsInt[Stack[StackPointer]] && RefToInt[Stack[StackPointer]] == 0);
+    goto failed;
+
+  failed:
+    call {:si_unique_call 29} Int(0);
+    call {:si_unique_call 30} Return();
+    goto finished;
+
+  finished:
+    call {:si_unique_call 31} Int(1);
+    call {:si_unique_call 32} Return();
+    return;
+}
+
+
